\begin{exercice*}
   Effectuer les calculs suivants, puis simplifier.   
      \begin{multicols}{3}
         \begin{enumerate}
            \begin{spacing}{2}
               \item $\dfrac23+\dfrac76$
               \item $\dfrac67-\dfrac3{14}$
               \item $\dfrac{38}{13}-\dfrac3{39}$
               \item $\dfrac{18}{46}+\dfrac{28}{23}$
               \item $\dfrac83-\dfrac26-\dfrac4{12}$
               \item $\dfrac12+\dfrac34+\dfrac58$
               \item $\dfrac34-4-\dfrac5{16}$
               \item $\dfrac{12}{49}+2-\dfrac97$
            \end{spacing}
         \end{enumerate}
      \end{multicols}   
\end{exercice*}

\begin{corrige}
   \ \\ [-5mm]
   \begin{enumerate}
      \item $\dfrac23+\dfrac76 =\dfrac46+\dfrac76 =\red \dfrac{11}6$ \bigskip
      \item $\dfrac67-\dfrac3{14} =\dfrac{12}{14}-\dfrac3{14} =\red \dfrac9{14}$ \bigskip
      \item $\dfrac{38}{13}-\dfrac3{39} =\dfrac{114}{39}-\dfrac3{39} =\dfrac{111}{39} =\red \dfrac{37}{13}$ \bigskip
      \item $\dfrac{18}{46}+\dfrac{28}{23} =\dfrac{9}{23}+\dfrac{28}{23} =\red \dfrac{37}{23}$ \bigskip
      \item $\dfrac83-\dfrac26-\dfrac4{12} =\dfrac{32}{12}-\dfrac{4}{12}-\dfrac{4}{12} =\dfrac{24}{12} =\red 2$ \bigskip
      \item $\dfrac12+\dfrac34+\dfrac58 =\dfrac48+\dfrac68+\dfrac58 =\red \dfrac{15}{8}$ \bigskip
      \item $\dfrac34-4-\dfrac5{16} =\dfrac{12}{16}-\dfrac{64}{16}-\dfrac{5}{16} =\red -\dfrac{57}{16}$ \bigskip
      \item $\dfrac{12}{49}+2-\dfrac97 =\dfrac{12}{49}+\dfrac{98}{49}-\dfrac{63}{49} =\red \dfrac{47}{49}$
   \end{enumerate}
\end{corrige}