\begin{exercice*}[Calculs d'expressions]
    Calculer.
    % \begin{multicols}2
        \begin{list}{}
            \item $ K = (-3+10)-(4-15)-(-12-8)$
            \item $ L = -33+2-(1-8) -(3+11)$
            \item $ M = -23-[40-(3-19)]$
            \item $ N = -6+[(11-18)-(33+6)-(5-11)]$
        \end{list}
    % \end{multicols}
\end{exercice*}
\begin{corrige}
    %\setcounter{partie}{0} % Pour s'assurer que le compteur de \partie est à zéro dans les corrigés
    \phantom{rrr}    
    \begin{multicols}2
        \begin{list}{}
            \item $ K=\underbrace{(-3+10)}_{7}-\underbrace{(4-15)}_{(-11)}-\underbrace{(-12-8)}_{(-20)}$\\
            $\phantom{A }=7-(-11)-(-20)$\\
            $\phantom{A }=7+11+20$\\
            $\phantom{A }=\mathbf{{\color{red}38}}$
            \item $ L=-33+2-\underbrace{(1-8)}_{(-7)} -\underbrace{(3+11)}_{14}$\\
            $\phantom{A }=-33+2-(-7)-14$\\
            $\phantom{A }=-33+2+7-14$\\
            $\phantom{A }=-47+9$\\
            $\phantom{A }=\mathbf{{\color{red}-38}}$
            \columnbreak
            \item $ M=-23-[40-\underbrace{(3-19)}_{-16}]$\\
            $\phantom{A }=-23-[40-(-16)]$\\
            $\phantom{A }=-23-[40+16)]$\\
            $\phantom{A }=-23-56$\\
            $\phantom{A }=\mathbf{{\color{red}-79}}$
            \item $ N=-6+[\underbrace{(11-18)}_{-7}-\underbrace{(33+6)}_{39}-\underbrace{(5-11)}_{(-6)}]$\\
            $\phantom{A }=-6+[-7-39-(-6)]$\\
            $\phantom{A }=-6+[-7-39+6]$\\
            $\phantom{A }=-6+[-46+6]$\\
            $\phantom{A }=-6-40$\\
            $\phantom{A }=\mathbf{{\color{red}-46}}$
        \end{list}
    \end{multicols}
\end{corrige}