\begin{exercice}
    Simplifier les expressions suivantes :
    \begin{enumerate}
       \item $A =a\times a$
       \item $B =b\times b\times b$
       \item $C =c\times c\times3$
       \item $D =9+d\times d\times d$
       \item $E =a\times a\times b\times3$
       \item $F =x\times x\times x-2\times y\times y$
       \item $G =(a+b)\times(a+b)$
       \item $H =(x+y)(x+y)(x+y)$
    \end{enumerate}
    \hrefMathalea{https://coopmaths.fr/mathalea.html?ex=5L16,s=2,s2=false,n=10,i=0&v=l}
 \end{exercice}
 
 \begin{corrige}
    \ \\ [-5mm]
    \begin{enumerate}
       \item $A =a\times a =\red a^2$
       \item $B =b\times b\times b =\red b^3$
       \item $C =c\times c\times3 =\red3c^2$
       \item $D =9+d\times d\times d =\red9+d^3$
       \item $E =a\times a\times b\times3 =\red3a^2b$
       \item $F =x\times x\times x-2\times y\times y =\red x^3-2y^2$
       \item $G =(a+b)\times(a+b) =\red(a+b)^2$
       \item $H =(x+y)(x+y)(x+y) =\red(x+y)^3$ \medskip
    \end{enumerate}
 \end{corrige}