\begin{exercice*}
    Soit $B=(x-5)^2 - 3(x-5)$
    \begin{enumerate}
        \item Factoriser $B$.
        \item Résoudre $B=0$.
    \end{enumerate}
\end{exercice*}
\begin{corrige}
    Soit $B=(x-5)^2 - 3(x-5)$
    
    \begin{enumerate}
        \item Factoriser $B$.
        
        $B=(x-5)\times[(x-5)-3]$\\
        $B=(x-5)\times(x-5-3)$\\
        $B=(x-5)\times(x-8)$\\
        $B=(x-5)(x-8)$
        \item Résoudre $B=0$.
        
        \ResolEquation[Produit,Facteurs,Entier,Simplification]{1}{-5}{1}{-8}
    \end{enumerate}
\end{corrige}