\begin{exercice*}
   Pour chaque cas, transformer la soustraction en addition puis effectuer le calcul.
   \begin{itemize}
      \item[] $A =(-12)-(+15)$
      \item[] $B =(-45)-(-41)$
      \item[] $C =(+32)-(+27)$
      \item[] $D =(-2,6)-(+2,7)$
      \item[] $E =(-1,4)-(-2,3)$
   \end{itemize}
   \hrefMathalea{https://coopmaths.fr/alea/?uuid=b6982&id=5R21&n=5&d=10&s=20&s2=false&cd=1&v=confeleve&v=eleve&title=&es=02110}
\end{exercice*}

\begin{corrige}
   \ \\ [-5mm]
   \begin{itemize}
      \def\item{}
      \item $A =(-12)-(+15)=(-12)+(-15)$ \\
         \qquad\; $=-(12+15) =\red -27$
      \item $B =(-45)-(-41) =(-45)+(+41)$ \\
         \qquad\; $=-(45-41) =\red -4$
      \item $C =(+32)-(+27) =(+32)+(-27)$ \\
         \qquad\; $=+(32-27) =\red 5$
      \item $D =(-2,6)-(+2,7) =(-2,6)+(-2,7)$ \\
         \qquad\; $=-(2,6+2,7) =\red -5,3$
      \item $E =(-1,4)-(-2,3) =(-1,4)+(+2,3)$ \\
         \qquad\; $=+(2,3-1,4) =\red 0,9$
   \end{itemize}
\end{corrige}
